src/lib/kuiper/Kuiper.Math.Silly.fsti
@@ -1,0 +1,24 @@
+module Kuiper.Math.Silly
+
+open FStar.Mul
+
+val lemma_nonneg_mul (x y : int)
+  : Lemma (requires x >= 0 /\ y >= 0)
+          (ensures x * y >= 0)
+
+val two_times_succ (x: int)
+  : Lemma (requires x >= 0)
+          (ensures 2 * (x + 1) = 2 * x + 2)
+
+val lemma_pos_times_pos (a b: pos)
+  : Lemma (a * b > 0)
+
+val lemma_nat_times_nat (a b: nat)
+  : Lemma (a * b >= 0)
+
+val lemma_sq_mono (a b : nat)
+  : Lemma (a <= b <==> a * a <= b * b)
+
+val lemma_sq_mono' (a b : nat)
+  : Lemma (a < b <==> a * a < b * b)
+
